Tests/DTLC/ValDemo.lean
@@ -2,11 +2,11 @@ import «Lp2lc».Active.DTLC.Def
 
 namespace Tests.DTLC.Sanity
 open Lp2lc.Active.DTLC
-open Lp2lc.Active.DTLC.Closed
+open Lp2lc.Active.DTLC.Symbolic
 
 namespace Val
 
-def idFn : ValAST :=
+def idFn : Val :=
   .fn fun x => .ref x
 
 end Val
